Full implementation of element modification through pointers

LLVM_DS_RBT/Insert/Alloc_Optimized/Insert_Opt.thy
@@ -1,191 +1,16 @@
 theory Insert_Opt
-  imports "../Insert"
+  imports 
+    "../Insert"
+    Balance_Opt
 begin
-
 
 context rbt_impl
 begin
 interpretation rbt_impl_deps .
 
-
-definition "balance_opt_case_1 n_p \<equiv> 
-  do {
-    n \<leftarrow> ll_load n_p;
-    set_color_p 0 n_p;
-    set_color_p 1 (rbt_node.left n);
-    set_color_p 1 (rbt_node.right n);
-    return n_p
-  }"
-
-
-definition "rotate_left n_p \<equiv>
-  do {
-    r_p \<leftarrow> right n_p;
-    rl_p \<leftarrow> left r_p;
-    set_left_p n_p r_p;
-    set_right_p rl_p n_p;
-    return r_p
-  }
-"
-
-
-definition "rotate_right n_p \<equiv>
-  do {
-    l_p \<leftarrow> left n_p;
-    lr_p \<leftarrow> right l_p;
-    set_right_p n_p l_p;
-    set_left_p lr_p n_p;
-    return l_p
-  }
-"
-                            
-definition "balance_opt_case_2 n_p \<equiv> 
-  do {
-    n2_p \<leftarrow> rotate_right n_p;
-    l_p \<leftarrow> left n2_p;
-    set_color_p 1 l_p;
-    return n2_p
-  }"
-
-
-definition "balance_opt_case_3 n_p \<equiv> 
-  do {
-    l_p \<leftarrow> left n_p;
-    l2_p \<leftarrow> rotate_left l_p;
-    set_left_p l2_p n_p;
-    n2_p \<leftarrow> rotate_right n_p;
-    set_color_p 1 l_p;
-    return n2_p
-  }"
-
-
-definition "balance_opt_case_4 n_p \<equiv> 
-  do {
-    n2_p \<leftarrow> rotate_left n_p;
-    r_p \<leftarrow> right n2_p;
-    set_color_p 1 r_p;
-    return n2_p
-  }"
-
-
-definition "balance_opt_case_5 n_p \<equiv> 
-  do {
-    r_p \<leftarrow> right n_p;
-    r2_p \<leftarrow> rotate_right r_p;
-    set_right_p r2_p n_p;
-    n2_p \<leftarrow> rotate_left n_p;
-    set_color_p 1 r_p;
-    return n2_p
-  }"
-
-find_theorems ll_matches_rbt htriple
-definition "balance_opt n_p \<equiv>
-  do {
-    if! ll_matches_rbt
-        (RP_Branch CP_Var 
-          (RP_Branch CP_R RP_Var RP_Var)
-          (RP_Branch CP_R RP_Var RP_Var)
-        ) n_p
-    then! balance_opt_case_1 n_p
-    else!
-    do {
-      n \<leftarrow> ll_load n_p;
-      l_p \<leftarrow> return rbt_node.left n;
-      r_p \<leftarrow> return rbt_node.right n;
-      if! ll_matches_rbt
-        (RP_Branch CP_R (RP_Branch CP_R RP_Var RP_Var) RP_Var) l_p
-      then! balance_opt_case_2 n_p
-      else! if! ll_matches_rbt 
-        (RP_Branch CP_R RP_Var (RP_Branch CP_R RP_Var RP_Var)) l_p
-      then! balance_opt_case_3 n_p
-      else! if! ll_matches_rbt 
-        (RP_Branch CP_R RP_Var (RP_Branch CP_R RP_Var RP_Var)) r_p
-      then! balance_opt_case_4 n_p
-      else! if! ll_matches_rbt 
-        (RP_Branch CP_R (RP_Branch CP_R RP_Var RP_Var) RP_Var) r_p
-      then! balance_opt_case_5 n_p
-      else! return n_p
-    }
-  }
-"
-
-lemmas [llvm_inline] =
-    balance_opt_case_1_def
-    balance_opt_case_2_def
-    balance_opt_case_3_def
-    balance_opt_case_4_def
-    balance_opt_case_5_def
-    rotate_left_def    
-    rotate_right_def
-
-lemmas [llvm_code] = balance_opt_def
-
-
-lemma balance_opt_correct [vcg_rules]:
-  "llvm_htriple
-  (
-    \<upharpoonleft>ll_bpto (RBT_NODE ci li ki vi ri) n_p **
-    rbt_assn l li **
-    rbt_assn r ri **   
-    \<upharpoonleft>key_assn k ki **
-    \<upharpoonleft>value_assn v vi **
-    color_assn color.B ci
-  )
-  (balance_opt n_p)
-  (\<lambda>res. rbt_assn (rbt_balance l k v r) res) 
-  "
-  unfolding 
-    balance_opt_def
-    balance_opt_case_1_def
-    balance_opt_case_2_def
-    balance_opt_case_3_def
-    balance_opt_case_4_def
-    balance_opt_case_5_def
-    rotate_left_def    
-    rotate_right_def
-
-  apply vcg
-  subgoal (*Case 1*)
-    apply (cases "(l, k, v, r)" rule: RBT_Impl.balance.cases)
-                        apply auto
-    apply vcg
-    done
-  subgoal (*Case 2+*)
-    apply vcg
-    subgoal (*Case 3*)
-      apply (cases "(l, k, v, r)" rule: RBT_Impl.balance.cases)
-                          apply auto
-       apply vcg
-      done
-    subgoal (*Case 4+*)
-      apply vcg
-      subgoal (*Case 4*)
-        apply (cases "(l, k, v, r)" rule: RBT_Impl.balance.cases)
-                            apply auto
-           apply vcg
-        done
-      subgoal (*Case 5+*)
-        apply vcg
-        subgoal (*Case 5*)
-          apply (cases "(l, k, v, r)" rule: RBT_Impl.balance.cases)
-                              apply auto
-           apply vcg
-          done
-        subgoal (*Case 6*)
-          apply (cases "(l, k, v, r)" rule: RBT_Impl.balance.cases)
-                              apply auto
-                              apply vcg
-          done
-        done
-      done
-    done
-  done
-
-
 definition "balance_black n_p c \<equiv> do { if c = 1 then balance_opt n_p else return n_p }"
 
 lemmas [llvm_inline] = balance_black_def
-
 
 partial_function (M) insert'_opt ::
   "'ki \<Rightarrow> 'vi \<Rightarrow> ('ki, 'vi) rbti \<Rightarrow> ('ki, 'vi) rbti llM" where
@@ -281,8 +106,6 @@ lemma insert_opt_correct [vcg_rules]:
   apply vcg
   done
 
-
 end
-
 
 end
