LLVM_DS_RBT/Load_Store_Example.thy
@@ -1,10 +1,11 @@
 theory Load_Store_Example
   imports 
     Extended_Assertion
-    Utilities_Extended_Assertion
+    Utilities_Ext
     Assertion_Tree_Lookup
     Lookup_Extended_Assertion
     "Insert/Alloc_Optimized/Insert_Opt_Ext"
+    "Delete/Alloc_Optimized/Delete_Opt_Ext"
     Extended_Assertion_Exceptions
     Load_Store
 begin
@@ -19,7 +20,7 @@ definition "example t k1 v1 k2 v2 \<equiv>
     t' \<leftarrow> insert_opt k2 v2 t;
     vp \<leftarrow> load p;
     store p v1;
-    return t'
+    return (t', vp)
   }
 "
 
@@ -34,7 +35,7 @@ lemma example_correct:
     \<upharpoonleft>value_assn v2 v2i
   )
   (example ti k1i v1i k2i v2i)
-  (\<lambda>res_ti. EXS res_t res_vi res_v.
+  (\<lambda>(res_ti, res_vi). EXS res_t res_v.
     rbt_assn_ext res_t {} res_ti **
     \<upharpoonleft>value_assn res_v res_vi ** \<upharpoonleft>key_assn k1 k1i **
     \<up>(rbt_of res_t = (rbt_update (rbt_insert k2 v2 (rbt_of t)) k1 v1))
@@ -48,11 +49,10 @@ lemma example_correct:
   apply vcg_compat
   apply (isep_drule drule: value_ex_join_ent, (auto)[3])
   apply simp
-  apply sepE
+  apply (sepEwith simp) 
   done
 
 method is_contains = match conclusion in "_ \<in> _" \<Rightarrow> succeed
-
 method test_filter = then_else is_contains \<open>solves auto\<close> succeed
 
 
@@ -67,9 +67,9 @@ lemma example_correct_2:
     \<upharpoonleft>value_assn v2 v2i
   )
   (example ti k1i v1i k2i v2i)
-  (\<lambda>res_ti. EXS res_t res_vi res_v.
+  (\<lambda>(res_ti, res_vi). EXS res_t res_v.
     rbt_assn_ext res_t {} res_ti **
-    \<upharpoonleft>value_assn res_v res_vi ** \<upharpoonleft>key_assn k1 k1i **
+    \<upharpoonleft>value_assn (the (rbt_lookup (rbt_insert k2 v2 (rbt_of t)) k1)) res_vi ** \<upharpoonleft>key_assn k1 k1i **
     \<up>(rbt_of res_t = (rbt_update (rbt_insert k2 v2 (rbt_of t)) k1 v1))
   )
   "
@@ -77,6 +77,52 @@ lemma example_correct_2:
   supply map_leD[elim]
   apply vcg
      apply auto[3]
+  apply vcg
+  apply vcg_compat
+  apply (sepEwith \<open>test_filter, auto?\<close> isep_dest: value_ex_join_ent)
+  apply simp
+  apply (sepEwith \<open>test_filter, auto?\<close> isep_dest: value_ex_join_ent)
+  done
+
+declare insert_opt_correct_ext'[vcg_rules del]
+
+definition "example2 t k1 v1 k2 v2 k3 \<equiv>
+  do {
+    p \<leftarrow> lookup_ptr t k1;
+    t' \<leftarrow> insert_opt k2 v2 t;
+    t'' \<leftarrow> delete_opt k3 t';
+    vp \<leftarrow> load p;
+    store p v1;
+    return (t'', vp)
+  }
+"
+
+lemma example2_correct:
+  "is_rbt (rbt_of t) \<Longrightarrow> rbt_lookup (rbt_of t) k1 \<noteq> None \<Longrightarrow> k1 \<noteq> k3 \<Longrightarrow>
+  llvm_htriple
+  (
+    rbt_assn_ext t {} ti **
+    \<upharpoonleft>key_assn k1 k1i **
+    \<upharpoonleft>key_assn k2 k2i **
+    \<upharpoonleft>key_assn k3 k3i **
+    \<upharpoonleft>value_assn v1 v1i **
+    \<upharpoonleft>value_assn v2 v2i
+  )
+  (example2 ti k1i v1i k2i v2i k3i)
+  (\<lambda>(res_ti, res_vi). EXS res_t res_v.
+    rbt_assn_ext res_t {} res_ti **
+    \<upharpoonleft>key_assn k1 k1i ** \<upharpoonleft>key_assn k3 k3i **
+    \<upharpoonleft>value_assn (the (rbt_lookup (rbt_delete k3 (rbt_insert k2 v2 (rbt_of t))) k1)) res_vi **
+    \<up>(rbt_of res_t = (rbt_update (rbt_delete k3 (rbt_insert k2 v2 (rbt_of t))) k1 v1))
+  )
+  "
+  unfolding example2_def
+  supply
+    map_leD[elim!]
+    is_rbt_def[simp]
+  apply vcg
+
+  apply auto[3]
   apply vcg
   apply vcg_compat
   apply (sepEwith \<open>test_filter, auto?\<close> isep_dest: value_ex_join_ent)
