LLVM_DS_RBT/Delete/Alloc_Optimized/Balance_Opt_LR_Ext.thy
@@ -1,0 +1,260 @@
+theory Balance_Opt_LR_Ext
+  imports 
+    "../../Free_Ext"
+    "../../Insert/Alloc_Optimized/Balance_Opt_Ext"
+    Balance_Opt_LR
+    Test
+begin
+
+
+context rbt_impl
+begin
+
+definition
+  "balance_left_valid c l k v r \<equiv>
+    \<exists>ln kn vn rn.
+    inv1 (Branch c (Branch color.B ln kn vn rn) k v r) \<and>
+    inv2 (Branch c (Branch color.B ln kn vn rn) k v r) \<and>
+    rbt_sorted (Branch c l k v r)
+  " 
+
+lemma balance_left_opt_ext_correct':
+  "
+  llvm_htriple
+  ( 
+    \<upharpoonleft>ll_bpto (RBT_NODE ci li ki vi ri) n_p **
+    rbt_assn_ext l {} li **
+    \<upharpoonleft>key_assn k ki **
+    \<upharpoonleft>value_assn v vi **
+    rbt_assn_ext r {} ri **
+    color_assn c ci **
+    \<up>(rbt_sorted (Branch c (rbt_of l) k v (rbt_of r))) ** \<up>(rbt_of l = rbt_del k' l_pre) ** \<up>(matches_rbt (RP_Branch CP_B RP_Var RP_Var) l_pre) ** 
+    \<up>(inv1 (Branch c l_pre k v (rbt_of r))) ** \<up>(inv2 (Branch c l_pre k v (rbt_of r)))
+  )
+  (balance_left_opt n_p)
+  (\<lambda>res_ti. EXS res_t.
+    rbt_assn_ext res_t {} res_ti **
+    \<up>(rbt_of res_t = rbt_balance_left (rbt_of l) k v (rbt_of r)) **
+    ctx(rbt_sorted (rbt_of res_t)) **
+    \<up>(ptr_of_key res_t res_ti = ptr_of_key (ATBranch c k v ci li ki vi ri l r) n_p)
+  )
+  "
+  unfolding 
+    balance_left_opt_def
+    bl_opt_case_1_def
+    bl_opt_case_2_def
+    bl_opt_case_3_def
+    rotate_left_def
+    rotate_right_def
+    left_def
+    right_def
+    balance_left_valid_def
+  supply sep_context_pureI[fri_red_rules]
+  apply vcg
+  subgoal (*case 1*)
+    apply (cases "(rbt_of l, k, v, rbt_of r)" rule: RBT_Impl.balance_left.cases)
+              apply auto
+     apply vcg
+    done
+  subgoal (*case 2+*)
+    apply vcg
+
+    subgoal (*case 2*)
+      apply (cases "(rbt_of l, k, v, rbt_of r)" rule: RBT_Impl.balance_left.cases)
+                apply auto
+       apply vcg
+      done
+    subgoal (*case 3+*)
+      apply vcg
+      subgoal (*case 3*)
+        apply (cases "(rbt_of l, k, v, rbt_of r)" rule: RBT_Impl.balance_left.cases)
+                  apply auto
+         supply ptr_of_key_simps[simp]
+         supply load_rbt_non_null[vcg_rules]
+         supply ptr_of_key_eqI[rule del]
+
+         supply rbt_greater_trans[intro]
+         supply rbt_less_trans[intro]
+
+        subgoal
+          apply vcg 
+          subgoal
+            apply vcg_compat 
+            apply (sepEwith auto)
+            apply simp
+            apply (sepwith simp)
+            done
+          done
+
+        subgoal 
+
+          apply vcg
+          subgoal
+            apply vcg_compat
+            apply sepE apply (sep | (auto)[])+
+            done
+          done
+        done
+      subgoal (*case 4*)
+        apply (cases "(rbt_of l, k, v, rbt_of r)" rule: RBT_Impl.balance_left.cases)
+                  apply (auto elim: matches_rbt.elims)
+        done
+      done
+    done
+  done
+
+definition
+  "balance_right_valid c l k v r \<equiv>
+    \<exists>ln kn vn rn.
+    inv1 (Branch c l k v (Branch color.B ln kn vn rn)) \<and>
+    inv2 (Branch c l k v (Branch color.B ln kn vn rn)) \<and>
+    rbt_sorted (Branch c l k v r)
+  "
+
+lemmas balance_left_opt_ext_correct[vcg_rules] = balance_left_opt_ext_correct'[simplified ctx_def]
+
+lemma balance_right_opt_ext_correct':
+  "
+  llvm_htriple
+  ( 
+    \<upharpoonleft>ll_bpto (RBT_NODE ci li ki vi ri) n_p **
+    rbt_assn_ext l {} li **
+    \<upharpoonleft>key_assn k ki **
+    \<upharpoonleft>value_assn v vi **
+    rbt_assn_ext r {} ri **
+    color_assn c ci **
+    \<up>(rbt_sorted (Branch c (rbt_of l) k v (rbt_of r))) ** \<up>(rbt_of r = rbt_del k' r_pre) ** \<up>(matches_rbt (RP_Branch CP_B RP_Var RP_Var) r_pre) ** 
+    \<up>(inv1 (Branch c (rbt_of l) k v r_pre)) ** \<up>(inv2 (Branch c (rbt_of l) k v r_pre))
+  )
+  (balance_right_opt n_p)
+  (\<lambda>res_ti. EXS res_t.
+    rbt_assn_ext res_t {} res_ti **
+    \<up>(rbt_of res_t = rbt_balance_right (rbt_of l) k v (rbt_of r)) **
+    ctx(rbt_sorted (rbt_of res_t)) **
+    \<up>(ptr_of_key res_t res_ti = ptr_of_key (ATBranch c k v ci li ki vi ri l r) n_p)
+  )
+  "
+  unfolding 
+    balance_right_opt_def
+    br_opt_case_1_def
+    br_opt_case_2_def
+    br_opt_case_3_def
+    rotate_left_def
+    rotate_right_def
+    left_def
+    right_def
+    balance_right_valid_def
+  supply sep_context_pureI[fri_red_rules]
+  apply vcg
+  subgoal (*case 1*)
+    apply (cases "(rbt_of l, k, v, rbt_of r)" rule: RBT_Impl.balance_right.cases)
+              apply auto
+     apply vcg
+    done
+  subgoal (*case 2+*)
+    apply vcg
+
+    subgoal (*case 2*)
+      apply (cases "(rbt_of l, k, v, rbt_of r)" rule: RBT_Impl.balance_right.cases)
+                apply auto
+       apply vcg
+      done
+    subgoal (*case 3+*)
+      apply vcg
+      subgoal (*case 3*)
+        apply (cases "(rbt_of l, k, v, rbt_of r)" rule: RBT_Impl.balance_right.cases)
+                  apply auto
+
+         supply ptr_of_key_simps[simp]
+         supply load_rbt_non_null[vcg_rules]
+         supply ptr_of_key_eqI[rule del]
+
+         supply rbt_greater_trans[intro]
+         supply rbt_less_trans[intro]
+
+        subgoal
+          apply vcg 
+          subgoal
+            apply vcg_compat 
+            apply (sepEwith auto)
+            apply simp
+            apply (sepwith simp)
+            done
+          done
+
+        subgoal 
+          apply vcg
+          subgoal
+            apply vcg_compat
+            apply sepE apply (sep | (auto)[])+
+            done
+          done
+        done
+      subgoal (*case 4*)
+        apply (cases "(rbt_of l, k, v, rbt_of r)" rule: RBT_Impl.balance_right.cases)
+                  apply (auto elim: matches_rbt.elims)
+        done
+      done
+    done
+  done
+
+lemmas balance_right_opt_ext_correct[vcg_rules] = balance_right_opt_ext_correct'[simplified ctx_def]
+
+
+
+lemma balance_left_opt_ext_combine_correct':
+  "
+  llvm_htriple
+  ( 
+    \<upharpoonleft>ll_bpto (RBT_NODE ci li ki vi ri) n_p **
+    rbt_assn_ext l {} li **
+    \<upharpoonleft>key_assn k ki **
+    \<upharpoonleft>value_assn v vi **
+    rbt_assn_ext r {} ri **
+    color_assn c ci **
+    \<up>(rbt_sorted (Branch c (rbt_of l) k v (rbt_of r))) **
+    \<up>(matches_rbt (RP_Branch CP_B RP_Var RP_Var) (rbt_of r))
+  )
+  (balance_left_opt n_p)
+  (\<lambda>res_ti. EXS res_t.
+    rbt_assn_ext res_t {} res_ti **
+    \<up>(rbt_of res_t = rbt_balance_left (rbt_of l) k v (rbt_of r)) **
+    ctx(rbt_sorted (rbt_of res_t)) **
+    \<up>(ptr_of_key res_t res_ti = ptr_of_key (ATBranch c k v ci li ki vi ri l r) n_p)
+  )
+  "
+  unfolding 
+    balance_left_opt_def
+    bl_opt_case_1_def
+    bl_opt_case_2_def
+    bl_opt_case_3_def
+    rotate_left_def
+    rotate_right_def
+    left_def
+    right_def
+    balance_left_valid_def
+  supply sep_context_pureI[fri_red_rules]
+  apply vcg
+  subgoal (*case 1*)
+    apply (cases "(rbt_of l, k, v, rbt_of r)" rule: RBT_Impl.balance_left.cases)
+              apply auto
+     apply vcg
+    done
+  subgoal (*case 2+*)
+    apply vcg
+
+    subgoal (*case 2*)
+      apply (cases "(rbt_of l, k, v, rbt_of r)" rule: RBT_Impl.balance_left.cases)
+                apply auto
+       apply vcg
+      done
+    apply vcg (*all other cases unreachable*)
+    done
+  done
+
+lemmas balance_left_opt_ext_combine_correct[vcg_rules] =
+  balance_left_opt_ext_combine_correct'[simplified ctx_def]
+
+end
+
+end
