LLVM_DS_RBT/Delete/Alloc_Optimized/Combine_Ext.thy
@@ -1,0 +1,226 @@
+theory Combine_Ext
+  imports
+    Combine_Opt
+    Balance_Opt_LR_Ext
+    "../../Assertion_Tree_Lookup"
+    "../../Utilities_Ext"
+begin
+
+context rbt_impl
+begin
+
+
+lemma disjoint_trees_map_add_graph [simp]:
+  assumes "rbt_of l |\<guillemotleft> k" and "k \<guillemotleft>| rbt_of r"
+  shows
+    "Map.graph (ptr_of_key l li ++ ptr_of_key r ri) =
+         Map.graph (ptr_of_key l li) \<union> Map.graph (ptr_of_key r ri)" 
+  unfolding map_add_def Map.graph_def
+  apply (rule equalityI)
+  subgoal by (auto split: option.splits)
+  subgoal apply (auto split: option.splits)
+    subgoal for a b x2
+    proof (cases k a rule: linorder_cases)
+      case less
+      with assms have "ptr_of_key l li a = None"  
+        using ptr_of_key_less_none rbt_less_trans by blast
+      moreover assume "ptr_of_key l li a = Some b"
+      ultimately show ?thesis by simp
+    next
+      case equal
+      with assms have "ptr_of_key l li a = None"  
+        using ptr_of_key_less_none rbt_less_trans by blast
+      moreover assume "ptr_of_key l li a = Some b"
+      ultimately show ?thesis by simp
+
+    next
+      case greater
+      with assms have "ptr_of_key r ri a = None"  
+        using ptr_of_key_greater_none rbt_greater_trans by blast
+      moreover assume "ptr_of_key r ri a = Some x2"
+      ultimately show ?thesis by simp
+    qed
+    done
+  done
+
+lemma combine_correct_ext':
+  "
+  llvm_htriple
+  (rbt_assn_ext l {} li ** rbt_assn_ext r {} ri **
+   \<up>(rbt_sorted (rbt_of l)) ** \<up>(rbt_sorted (rbt_of r)) ** \<up>(rbt_of l |\<guillemotleft> k \<and> k \<guillemotleft>| rbt_of r))
+  (combine_opt li ri)
+  (\<lambda>res_ti. EXS res_t.
+    rbt_assn_ext res_t {} res_ti **
+    ctx(rbt_of res_t = rbt_combine (rbt_of l) (rbt_of r)) **
+    ctx(rbt_sorted (rbt_of res_t)) **
+    \<up>(ptr_of_key res_t res_ti = ptr_of_key l li ++ ptr_of_key r ri)
+  )
+  "
+  supply ptr_of_key_simps[simp]
+  supply sep_context_pureI[fri_red_rules]
+proof(induction "rbt_of l" "rbt_of r" arbitrary: l r li ri rule: RBT_Impl.combine.induct)
+  case 1
+  then show ?case
+    apply (subst combine_opt.simps)
+    apply vcg
+    done
+next
+  case (2 v va vb vc vd)
+  then show ?case
+    apply (subst combine_opt.simps)
+    apply vcg
+    done
+next
+  case (3 a k x b c s y d)
+  note 3(1)[simplified ctx_def, vcg_rules]
+
+  from 3(2-3) show ?case
+    supply RBT_Impl.combine.simps[simp del]
+
+    apply (subst combine_opt.simps)
+    apply vcg
+    subgoal
+      apply resolve_rbt_pat_mat
+      subgoal
+        supply rbt_sorted.simps[simp del]
+        apply vcg
+        apply vcg_compat
+        subgoal
+          apply sepE
+           apply (auto simp add: RBT_Impl.combine.simps)[] 
+
+          apply sep
+           apply simp
+           apply (rule combine_rbt_sorted)
+          using rbt_sorted.simps apply fast+
+            apply auto[2]
+
+          apply (sepwith auto)
+          apply simp
+          apply (sepwith simp)
+
+          done
+        done
+      done
+    subgoal
+      supply rbt_sorted.simps[simp del]
+      apply vcg
+      apply vcg_try_solve
+       apply (cases "rbt_combine b c")
+        apply (auto simp add: RBT_Impl.combine.simps split: color.splits)[2]
+      apply vcg_compat
+      apply sep
+
+       apply simp
+       apply (rule combine_rbt_sorted)
+      using rbt_sorted.simps apply fast+
+        apply auto[2]
+
+      apply sep  
+       apply simp
+       apply (auto simp: rbt_sorted.simps)[1]
+
+      apply sep
+      done
+    done
+next
+  case (4 a k x b c s y d)
+  note 4(1)[simplified ctx_def, vcg_rules]
+
+  from 4(2-3) show ?case
+    supply RBT_Impl.combine.simps[simp del]
+
+    apply (subst combine_opt.simps)
+    apply vcg
+    subgoal
+      apply resolve_rbt_pat_mat
+      supply rbt_sorted.simps[simp del]
+      apply vcg
+      apply vcg_compat
+      subgoal
+        apply sepE
+         apply (auto simp add: RBT_Impl.combine.simps)[] 
+
+        apply sep
+         apply simp
+         apply (rule combine_rbt_sorted)
+        using rbt_sorted.simps apply fast+
+          apply auto[2]
+
+        apply (sepwith auto)
+        apply simp
+        apply (sepwith simp)
+
+        done
+      done
+
+    subgoal
+      supply  
+        rbt_less_trans[intro]
+        rbt_greater_trans[intro]
+        combine_rbt_greater[intro]
+        combine_rbt_less[intro]
+      apply vcg
+      apply vcg_compat
+      apply sepE
+       apply (cases "rbt_combine b c")
+        apply (auto simp add: RBT_Impl.combine.simps split: color.splits)[2]
+      apply sep
+
+       apply simp
+      apply sep
+
+       apply simp 
+       apply (subst ptr_of_key_simps(4), (auto)[])+
+       apply auto[1]
+
+      apply sep
+      done
+    done
+  next
+    case (5 va vb vc vd b k x c)
+    note 5(1)[simplified ctx_def, vcg_rules]
+    note load_rbt_non_null[vcg_rules]
+    from 5(2-3) show ?case
+      apply (subst combine_opt.simps)
+      apply vcg
+      apply vcg_compat
+      subgoal
+        supply  
+          rbt_less_trans[intro]
+          rbt_greater_trans[intro]
+          combine_rbt_greater[intro]
+          combine_rbt_less[intro]
+
+        apply (sepEwith force)
+        apply simp 
+        apply (sepwith simp)
+        done 
+      done
+  next
+    case (6 a k x b va vb vc vd)
+    note 6(1)[simplified ctx_def, vcg_rules]
+    note load_rbt_non_null[vcg_rules]
+    from 6(2-3) show ?case
+      apply (subst combine_opt.simps)
+      apply vcg
+      apply vcg_compat
+      subgoal
+        supply  
+          rbt_less_trans[intro]
+          rbt_greater_trans[intro]
+          combine_rbt_greater[intro]
+          combine_rbt_less[intro]
+
+        apply (sepEwith force)
+        apply simp 
+        apply (sepwith simp)
+        done 
+      done
+  qed
+
+lemmas combine_correct_ext[vcg_rules] = combine_correct_ext'[simplified ctx_def]
+
+end
+
+end
