LLVM_DS_RBT/Delete/Alloc_Optimized/Delete_Opt_Ext.thy
@@ -1,0 +1,156 @@
+theory Delete_Opt_Ext
+  imports 
+    Delete_Opt
+    Balance_Opt_LR_Ext
+    Combine_Ext
+    "../../Assertion_Tree_Lookup"
+    "../../Utilities_Ext"
+begin
+
+context rbt_impl
+begin
+
+abbreviation "is_rbt_node t \<equiv> inv1 t \<and> inv2 t \<and> rbt_sorted t"
+
+lemma del_opt_correct_ext':
+  "
+  llvm_htriple
+  (rbt_assn_ext t {} ti ** \<upharpoonleft>key_assn k ki ** \<up>(is_rbt_node (rbt_of t)))
+  (del_opt ki ti)
+  (\<lambda>ti_res. EXS t_res.
+    rbt_assn_ext t_res {} ti_res **
+    \<upharpoonleft>key_assn k ki **
+    \<up>(rbt_of t_res = rbt_del_ad k (rbt_of t)) **
+    ctx(rbt_sorted (rbt_of t_res)) **
+    \<up>((ptr_of_key t ti)(k := None) \<subseteq>\<^sub>m ptr_of_key t_res ti_res)
+  )
+  "
+  supply sep_context_pureI[fri_red_rules]
+proof(induct k "rbt_of t" arbitrary: t ki ti rule: rbt_del_ad.induct)
+  case (1 k)
+  then show ?case
+    apply (subst del_opt.simps)
+    apply vcg
+    done
+next
+  case (2 k c l kc vc r)
+
+  from 2(5) show ?case
+    apply (subst del_opt.simps)
+    supply load_rbt_non_null[vcg_rules]
+    apply vcg
+
+    subgoal for al ar ci li ki vi ri asf ra sa (*k < kc*)
+      apply (cases ra)
+      subgoal (*ra = 0*)
+        supply 2(2)[simplified ctx_def, vcg_rules]
+
+        supply rbt_del_ad_correct[simp]
+        supply rbt_del_rbt_less[intro]
+        supply rbt_del_rbt_sorted[intro]
+
+        supply ptr_of_key_simps[simp]
+
+        apply vcg 
+        apply vcg_compat
+        apply (sepEwith auto)
+
+        apply simp
+        apply sep
+        done
+
+      subgoal (*ra = 1*)
+        supply 2(1)[simplified ctx_def, vcg_rules]
+        supply rbt_del_rbt_less[simp]
+        supply rbt_del_ad_correct[simp]
+        supply ptr_of_key_simps[simp]
+
+        apply vcg
+        done
+      done
+
+    subgoal for al ar ci li ki vi ri asf ra s (*kc \<le> k*)
+      apply vcg
+      subgoal for rb sa (*kc < k*)
+              apply (cases rb)
+      subgoal (*rb = 0*)
+        supply 2(4)[simplified ctx_def, vcg_rules]
+
+        supply rbt_del_ad_correct[simp]
+        supply rbt_del_rbt_greater[intro]
+        supply rbt_del_rbt_sorted[intro]
+
+        supply ptr_of_key_simps[simp]
+
+        apply vcg 
+        apply vcg_compat
+        apply (sepEwith auto)
+
+        apply simp
+        apply sep
+        done
+
+      subgoal (*rb = 1*)
+        supply 2(3)[simplified ctx_def, vcg_rules]
+        supply rbt_del_rbt_greater[simp]
+        supply rbt_del_ad_correct[simp]
+        supply ptr_of_key_simps[simp]
+
+        apply vcg
+        done
+      done
+      subgoal (*kc = k*)
+        supply ptr_of_key_simps[simp]
+        apply vcg
+      done
+    done
+  done
+qed
+
+lemmas del_opt_ext_correct = del_opt_correct_ext'[simplified ctx_def rbt_del_ad_correct]
+
+lemma delete_opt_ext_correct [vcg_rules]:
+"
+  llvm_htriple
+  (\<upharpoonleft>key_assn k ki ** rbt_assn_ext t {} ti ** \<up>(is_rbt_node (rbt_of t)))
+  (delete_opt ki ti)
+  (\<lambda>res_ti. EXS res_t.
+    rbt_assn_ext res_t {} res_ti **
+    \<upharpoonleft>key_assn k ki **
+    \<up>(rbt_of res_t = (rbt_delete k (rbt_of t))) **
+    \<up>(rbt_sorted (rbt_of res_t)) **
+    \<up>((ptr_of_key t ti)(k := None) \<subseteq>\<^sub>m ptr_of_key res_t res_ti)
+  )
+"
+  unfolding delete_opt_def rbt_delete_def paint_def
+  supply 
+    del_opt_ext_correct[vcg_rules] 
+    load_rbt_non_null[vcg_rules]    
+    
+  apply vcg
+  subgoal
+    apply vcg_compat
+    apply (sepEwith auto)
+     (*rbt_of =*)
+     apply (cases "rbt_del k (rbt_of t)") 
+      apply simp_all
+
+    apply (sepwith simp)
+    subgoal using rbt_sorted.simps(2) by metis (*rbt_sorted*)
+
+    apply sep
+    subgoal (*ptr_of_key relation*)
+      apply (simp add: ptr_of_key_simps)
+      apply (subst ptr_of_key_simps(4))
+       apply (simp only: rbt_of.simps)
+      using rbt_sorted.simps(2) apply metis
+      apply simp
+      done
+
+    apply sep
+    done
+  done
+
+end
+
+end
