LLVM_DS_RBT/Free_Ext.thy
@@ -1,0 +1,36 @@
+theory Free_Ext
+  imports 
+    Extended_Assertion
+    Free
+begin
+
+context rbt_impl
+begin
+
+lemma free_correct_ext [vcg_rules]:
+  "
+    llvm_htriple
+    (rbt_assn_ext t {} ti)
+    (free ti)
+    (\<lambda>_. \<box>)
+  "
+proof(induction t arbitrary: ti)
+  case ATEmpty
+  then show ?case
+    apply (subst free.simps)
+    apply vcg
+    done
+next
+  case (ATBranch c k v ci li ki vi ri al ar)
+
+  note [vcg_rules] = ATBranch.IH
+  
+  then show ?case
+    apply (subst free.simps)
+    apply vcg
+    done
+qed
+
+end
+
+end
