LLVM_DS_RBT/Insert/Alloc_Optimized/Balance_Opt_Ext.thy
@@ -1,0 +1,74 @@
+theory Balance_Opt_Ext
+  imports 
+    Balance_Opt
+    "../../Assertion_Tree_Lookup"
+    "../../Utilities_Ext"
+begin
+
+context rbt_impl
+begin
+
+lemma balance_opt_correct_ext [vcg_rules]:
+  "llvm_htriple
+  (
+    rbt_assn_ext (ATBranch color.B k v ci li ki vi ri l r) {} ti ** \<up>(rbt_sorted (rbt_of (ATBranch color.B k v ci li ki vi ri l r)))
+  )
+  (balance_opt ti)
+  (\<lambda>res. EXS res_t. rbt_assn_ext res_t {} res **
+    \<up>(rbt_of res_t = rbt_balance (rbt_of l) k v (rbt_of r)) **
+    \<up>(rbt_sorted (rbt_of res_t)) **
+    \<up>(ptr_of_key res_t res = ptr_of_key (ATBranch color.B k v ci li ki vi ri l r) ti)  
+  )
+  "
+  unfolding 
+    balance_opt_def
+    balance_opt_case_1_def
+    balance_opt_case_2_def
+    balance_opt_case_3_def
+    balance_opt_case_4_def
+    balance_opt_case_5_def
+    rotate_left_def    
+    rotate_right_def
+    right_def
+    left_def
+  supply rbt_greater_trans[intro] rbt_less_trans[intro]
+  apply vcg
+  subgoal (*Case 1*)
+    apply (cases "(rbt_of l, k, v, rbt_of r)" rule: RBT_Impl.balance.cases)
+    apply auto
+    apply vcg
+    done
+  subgoal (*Case 2+*)
+    apply vcg
+    subgoal (*Case 2*)
+      apply (cases "(rbt_of l, k, v, rbt_of r)" rule: RBT_Impl.balance.cases)
+      apply auto
+      apply vcg
+      done
+    subgoal (*Case 3+*)
+      apply vcg
+      subgoal (*Case 3*)
+        apply (cases "(rbt_of l, k, v, rbt_of r)" rule: RBT_Impl.balance.cases)
+        apply auto 
+        apply vcg
+        done
+      subgoal (*Case 4+*)
+        apply vcg
+        subgoal (*Case 4*)
+          apply (cases "(rbt_of l, k, v, rbt_of r)" rule: RBT_Impl.balance.cases)
+          apply auto
+          apply vcg
+          done
+        subgoal (*Case 5*)
+          apply (cases "(rbt_of l, k, v, rbt_of r)" rule: RBT_Impl.balance.cases)
+          apply auto
+          apply vcg
+          done
+        done
+      done
+    done
+  done
+
+end
+
+end
