LLVM_DS_RBT/Insert/Alloc_Optimized/Insert_Opt_Ext.thy
@@ -1,73 +1,13 @@
 theory Insert_Opt_Ext
   imports
     Insert_Opt  
-    "../../Utilities_Extended_Assertion"
+    Balance_Opt_Ext
+    "../../Utilities_Ext"
     "../../Assertion_Tree_Lookup"
 begin
 
 context rbt_impl
 begin
-
-lemma balance_opt_correct_ext [vcg_rules]:
-  "llvm_htriple
-  (
-    rbt_assn_ext (ATBranch color.B k v ci li ki vi ri l r) {} ti ** \<up>(rbt_sorted (rbt_of (ATBranch color.B k v ci li ki vi ri l r)))
-  )
-  (balance_opt ti)
-  (\<lambda>res. EXS res_t. rbt_assn_ext res_t {} res **
-    \<up>(rbt_of res_t = rbt_balance (rbt_of l) k v (rbt_of r)) **
-    \<up>(rbt_sorted (rbt_of res_t)) **
-    \<up>(ptr_of_key res_t res = ptr_of_key (ATBranch color.B k v ci li ki vi ri l r) ti)  
-  )
-  "
-  unfolding 
-    balance_opt_def
-    balance_opt_case_1_def
-    balance_opt_case_2_def
-    balance_opt_case_3_def
-    balance_opt_case_4_def
-    balance_opt_case_5_def
-    rotate_left_def    
-    rotate_right_def
-    right_def
-    left_def
-  supply rbt_greater_trans[intro] rbt_less_trans[intro]
-  apply vcg
-  subgoal (*Case 1*)
-    apply (cases "(rbt_of l, k, v, rbt_of r)" rule: RBT_Impl.balance.cases)
-                        apply auto
-    apply vcg
-    done
-  subgoal (*Case 2+*)
-    apply vcg
-    subgoal (*Case 2*)
-      apply (cases "(rbt_of l, k, v, rbt_of r)" rule: RBT_Impl.balance.cases)
-                          apply auto
-       apply vcg
-      done
-    subgoal (*Case 3+*)
-      apply vcg
-      subgoal (*Case 3*)
-        apply (cases "(rbt_of l, k, v, rbt_of r)" rule: RBT_Impl.balance.cases)
-                            apply auto 
-           apply vcg
-        done
-      subgoal (*Case 4+*)
-        apply vcg
-        subgoal (*Case 4*)
-          apply (cases "(rbt_of l, k, v, rbt_of r)" rule: RBT_Impl.balance.cases)
-                              apply auto
-           apply vcg
-          done
-        subgoal (*Case 5*)
-          apply (cases "(rbt_of l, k, v, rbt_of r)" rule: RBT_Impl.balance.cases)
-                              apply auto
-                              apply vcg
-          done
-        done
-      done
-    done
-  done
 
 lemma insert'_opt_correct_ext:
   "
@@ -112,7 +52,7 @@ next
     done
 qed
 
-lemma insert_opt_correct_ext [vcg_rules]:
+lemma insert_opt_correct_ext' [vcg_rules]:
   "
     llvm_htriple
     (rbt_assn_ext t {} ti ** \<upharpoonleft>key_assn k ki ** \<upharpoonleft>value_assn v vi ** \<up>(rbt_sorted (rbt_of t)))
@@ -146,6 +86,22 @@ lemma insert_opt_correct_ext [vcg_rules]:
   subgoal by simp
   subgoal by blast
   subgoal by (auto dest!: ptr_of_key_subsetD)
+  done
+
+
+lemma insert_opt_correct_ext [vcg_rules]:
+  "
+    llvm_htriple
+    (rbt_assn_ext t {} ti ** \<upharpoonleft>key_assn k ki ** \<upharpoonleft>value_assn v vi ** \<up>(is_rbt (rbt_of t)))
+    (insert_opt ki vi ti)
+    (\<lambda>res_ti. EXS res_t.
+      rbt_assn_ext res_t {} res_ti **
+      \<up>(rbt_of res_t = rbt_insert k v (rbt_of t)) **
+      \<up>(is_rbt (rbt_of res_t)) **
+      \<up>(ptr_of_key t ti \<subseteq>\<^sub>m ptr_of_key res_t res_ti)
+    )
+  "
+  apply vcg
   done
 
 end
