LLVM_DS_RBT/Separation_Logic_Solver/Shifts.thy
@@ -4,7 +4,11 @@ begin
 
 
 lemma shift_entails_prem: "(As ** A) ** Bs \<turnstile> Q \<Longrightarrow> As ** A ** Bs \<turnstile> Q"
-  by simp 
+  by simp
+
+
+lemma shift_entails_conc: "P \<turnstile> (As ** A) ** Bs \<Longrightarrow> P  \<turnstile> As ** A ** Bs"
+  by simp
 
 
 lemma shift_frame_prem: "((As ** A) ** Bs) -- PR \<tturnstile> Q -- QR \<Longrightarrow> (As ** A ** Bs) -- PR \<tturnstile> Q -- QR"
@@ -14,10 +18,13 @@ lemma shift_frame_prem: "((As ** A) ** Bs) -- PR \<tturnstile> Q -- QR \<Longrig
 lemma shift_frame_conc: "P -- PR \<tturnstile> ((As ** A) ** Bs) -- QR \<Longrightarrow> P -- PR \<tturnstile> (As ** A ** Bs) -- QR"
   by simp
 
+method_setup no_inst_rule = 
+  \<open>Attrib.thms >> (fn thms => fn ctxt => SIMPLE_METHOD' (match_tac ctxt thms THEN_ALL_NEW Goal.norm_hhf_tac ctxt))\<close>
 
-method all_entails_prem_shifts methods M = append \<open>M\<close> \<open>rule shift_entails_prem, all_entails_prem_shifts M\<close>
-method all_frame_prem_shifts methods M = append \<open>M\<close> \<open>rule shift_frame_prem, all_frame_prem_shifts M\<close>
-method all_frame_conc_shifts methods M = append \<open>M\<close> \<open>rule shift_frame_conc, all_frame_conc_shifts M\<close>
+method all_entails_prem_shifts methods M = append \<open>M\<close> \<open>no_inst_rule shift_entails_prem, all_entails_prem_shifts M\<close>
+method all_entails_conc_shifts methods M = append \<open>M\<close> \<open>no_inst_rule shift_entails_conc, all_entails_conc_shifts M\<close>
+method all_frame_prem_shifts methods M = append \<open>M\<close> \<open>no_inst_rule shift_frame_prem, all_frame_prem_shifts M\<close>
+method all_frame_conc_shifts methods M = append \<open>M\<close> \<open>no_inst_rule shift_frame_conc, all_frame_conc_shifts M\<close>
 
 
 end
